Sure, here's a translation of the provided exercises:

### Exercise 5.3.1

Below is the grammar involving the operators + and integer or floating-point operands. The distinction between floating-point numbers is whether they contain a decimal point.

    E -> E + T | T
    T -> num.num | num
    
1. Provide an SDD to determine the type of each term T and expression E.
2. Extend the obtained SDD to allow it to convert expressions into postfix notation. Use a unary operator intToFloat to convert an integer into an equivalent floating-point number.

#### Solution

1.

    <table>
        <thead>
            <tr>
                <th></th>
                <th>Production</th>
                <th>Semantic Rule</th>
            </tr>
        </thead>
        <tbody>
            <tr>
                <td>1)</td>
                <td>E -> E_1 + T</td>
                <td>E.type = E_1.type === float || T.type === float ? float : int</td>
            </tr>
            <tr>
                <td>2)</td>
                <td>E -> T</td>
                <td>E.type = T.type</td>
            </tr>
            <tr>
                <td>3)</td>
                <td>T -> num.num</td>
                <td>T.type = float</td>
            </tr>
            <tr>
                <td>4)</td>
                <td>T -> num</td>
                <td>T.type = int</td>
            </tr>
        </tbody>
    </table>


### Exercise 5.3.2

Provide an SDD to translate an infix expression with + and * into an expression without redundant parentheses. For example, because both operators are left-associative and * has higher precedence than +, ((a*(b+c))*(d)) can be translated as a*(b+c)*d.

#### Solution

Definitions:

- wrapped: Whether the expression has outer parentheses.
- precedence: Assign 0 to +, 1 to *, 2 to (), and 3 to single digits. If the expression has outer parentheses, it is the precedence of the last operator after removing parentheses; otherwise, it is the precedence of the last operator in the expression.
- expr: The expression.
- cleanExpr: The expression without redundant parentheses.

<table>
    <thead>
        <tr>
            <th></th>
            <th>Production</th>
            <th>Semantic Rule</th>
        </tr>
    </thead>
    <tbody>
        <tr>
            <td>1)</td>
            <td>L -> En</td>
            <td>
                L.cleanExpr = E.wrapped ? E.cleanExpr : E.expr
            </td>
        </tr>
        <tr>
            <td>2)</td>
            <td>E -> E_1 + T</td>
            <td>
                E.wrapped = false<br/>
                E.precedence = 0<br/>
                E.expr = E_1.expr || "+" || T.expr<br/>
                E.cleanExpr = (E_1.wrapped ? E_1.cleanExpr : E_1.expr) || "+" || (T.wrapped ? T.cleanExpr : T.expr)
            </td>
        </tr>
        <tr>
            <td>3)</td>
            <td>E -> T</td>
            <td>
                E.wrapped = T.wrapped<br/>
                E.precedence = T.precedence<br/>
                E.expr = T.expr</br>
                E.cleanExpr = T.cleanExpr
            </td>
        </tr>
        <tr>
            <td>4)</td>
            <td>T -> T_1 * F</td>
            <td>
                T.wrapped = false<br/>
                T.precedence = 1<br/>
                T.expr = T_1.expr || "*" || F.expr<br/>
                T.cleanExpr = (T_1.wrapped && T_1.precedence >= 1 ? T_1.cleanExpr : T_1) || * || (F.wrapped && F.precedence >= 1 ? F.cleanExpr : F.expr)
            </td>
        </tr>
        <tr>
            <td>5)</td>
            <td>T -> F</td>
            <td>
                T.wrapped = F.wrapped<br/>
                T.precedence = F.precedence<br/>
                T.expr = F.expr<br/>
                T.cleanExpr = F.cleanExpr
            </td>
        </tr>
        <tr>
            <td>6)</td>
            <td>F -> (E)</td>
            <td>
                F.wrapped = true<br/>
                F.precedence = E.precedence<br/>
                F.expr = "(" || E.expr || ")"<br/>
                F.cleanExpr = E.expr
            </td>
        </tr>
        <tr>
            <td>7)</td>
            <td>F -> digit</td>
            <td>
                F.wrapped = false<br/>
                F.precedence = 3<br/>
                F.expr = digit<br/>
                F.cleanExpr = digit
            </td>
        </tr>
    </tbody>
</table>

 
### Exercise 5.3.3

Provide an SDD for differentiating an expression like x*(3*x+x*x). The expression involves operators + and *, variable x, and constants. Assume no simplifications are performed, meaning, for instance, 3*x will be translated to 3*1+0*x.
