# Section 4.4 Exercises

### 4.4.1

Design a predictive parser for each of the grammars below and provide the predictive parsing table. You may need to factor the grammar or eliminate left recursion first.

Grammars from Exercise 4.2.2 (items 1 - 7):

#### Solution

1. **S -> 0 S 1 | 0 1**

    Step 1: Factor the grammar
    
        S -> 0 A
        A -> S 1 | 1

    Step 2: Eliminate left recursion
    
        S -> 0 A
        A -> 0 A 1 | 1
    
    Step 3: Predictive parsing table
    
    <table>
        <thead>
            <tr>
                <th rowspan="2">Non-terminal</th>
                <th colspan="3">Input Symbol</th>
            </tr>
            <tr>
                <th>0</th>
                <th>1</th>
                <th>$</th>
            </tr>
        </thead>
        <tbody>
            <tr>
                <th>S</th>
                <td>S -> 0 A</td>
                <td></td>
                <td></td>
            </tr>
            <tr>
                <th>A</th>
                <td>A -> 0 A 1</td>
                <td>A -> 1</td>
                <td></td>
            </tr>
        </tbody>
    </table>

2. **S -> + S S | * S S | a**
    
    Step 1: No factoring needed
    
    Step 2: No left recursion
    
    Step 3: Predictive parsing table
    
    <table>
        <thead>
            <tr>
                <th rowspan="2">Non-terminal</th>
                <th colspan="4">Input Symbol</th>
            </tr>
            <tr>
                <th>+</th>
                <th>*</th>
                <th>a</th>
                <th>$</th>
            </tr>
        </thead>
        <tbody>
            <tr>
                <th>S</th>
                <td>S -> + S S</td>
                <td>S -> * S S</td>
                <td>S -> a</td>
                <td></td>
            </tr>
        </tbody>
    </table>
    
3. **S -> S (S) S | ε**

    Step 1: No factoring needed

    Step 2: Eliminate left recursion
    
        S -> A
        A -> (S) S A | ε
        
    Step 3: Predictive parsing table
    
    <table>
        <thead>
            <tr>
                <th rowspan="2">Non-terminal</th>
                <th colspan="3">Input Symbol</th>
            </tr>
            <tr>
                <th>(</th>
                <th>)</th>
                <th>$</th>
            </tr>
        </thead>
        <tbody>
            <tr>
                <th>S</th>
                <td>S -> A</td>
                <td>S -> A</td>
                <td>S -> A</td>
            </tr>
            <tr>
                <th>A</th>
                <td>A -> (S) S A<br/>A -> ε</td>
                <td>A -> ε</td>
                <td>A -> ε</td>
            </tr>
        </tbody>
    </table>

4. **S -> S + S | S S | (S) | S * | a**
        
    Step 1: Factor the grammar
    
        S -> SA | (S) | a
        A -> +S | S | *
        
    Further factor out terminal symbols:
    
        S -> SA | T
        A -> +S | S | *
        T -> (S) | a  
    
    Step 2: Eliminate left recursion
    
        i = 1
                S -> TB
                B -> AB | ε
                
        i = 2
            j = 1
                A -> +S | TB | *
                
        i = 3
            j = 1
                No need to process
            j = 2
                No need to process
                
    Final productions:
    
        S -> TB
        B -> AB | ε
        A -> +S | TB | *
        T -> (S) | a  

    Step 3: First and follow sets
    
        first(T) = [(, a]
        first(A) = [+, *] + first(T) =[+, *, (, a]
        first(B) = [ε] + first(A) = [ε, +, *, (, a]
        first(S) = first(T) = [(, a]
    
        follow(T) = [$, +, *, (, a]
        follow(A) = [$, +, *, (, ), a]
        follow(B) = [$]
        follow(S) = [$, +, *, (, ), a]

    Step 4: Predictive parsing table
    
    <table>
        <thead>
            <tr>
                <th rowspan="2">Non-terminal</th>
                <th colspan="6">Input Symbol</th>
            </tr>
            <tr>
                <th>(</th>
                <th>)</th>
                <th>+</th>
                <th>*</th>
                <th>a</th>
                <th>$</th>
            </tr>
        </thead>
        <tbody>
            <tr>
                <th>S</th>
                <td>S -> TB</td>
                <td></td>
                <td></td>
                <td></td>
                <td>S -> TB</td>
                <td></td>
            </tr>
            <tr>
                <th>B</th>
                <td>B -> AB</td>
                <td></td>
                <td>B -> AB</td>
                <td>B -> AB</td>
                <td>B -> AB</td>
                <td>B -> ε</td>
            </tr>
            <tr>
                <th>A</th>
                <td>A -> TB</td>
                <td></td>
                <td>A -> +S</td>
                <td>A -> *</td>
                <td>A -> TB</td>
                <td></td>
            </tr>
            <tr>
                <th>T</th>
                <td>T -> (S)</td>
                <td></td>
                <td></td>
                <td></td>
                <td>T -> a </td>
                <td></td>
            </tr>
        </tbody>
    </table>

5. **S -> (L) | a** and **L -> L, S | S**

    Step 1: No factoring needed
    
    Step 2: Eliminate left recursion
    
        S -> (L) | a
        L -> SA
        A -> ,SA | ε
    
    Step 3: Predictive parsing table

6. **Grammar for boolean expressions:**

    ```
    bexpr -> bexpr or bterm | bterm
    bterm -> bterm and bfactor | bfactor
    bfactor -> not bfactor | ( bexpr ) | true | false
    ```

    Step 1: No factoring needed

    Step 2: Eliminate left recursion
    
    ```
    bexpr -> bterm bexpr'
    bexpr' -> or bterm bexpr' | ε
    bterm -> bfactor bterm'
    bterm' -> and bfactor bterm' | ε
    bfactor -> not bfactor | (bexpr) | true | false
    ```
    
    Step 3: First and follow sets
    
    ```
    first(bexpr) = first(bterm) = first(bfactor) = [not, (, true, false]
    first(bexpr') = [or, ε]
    first(bterm') = [and, ε]
    
    follow(bexpr) = follow(bexpr') = [), $]
    follow(bterm) = follow(bterm') = [or, $]
    follow(bfactor) = [and, $]
   
    ````
    
    Step 4: Predictive parsing table
    
    <table>
        <thead>
            <tr>
                <th rowspan="2">Non-terminal</th>
                <th colspan="8">Input Symbol</th>
            </tr>
            <tr>
                <th>and</th>
                <th>or</th>
                <th>not</th>
                <th>(</th>
                <th>)</th>
                <th>true</th>
                <th>false</th>
                <th>$</th>
            </tr>
        </thead>
        <tbody>
            <tr>
                <th>bexpr</th>
                <td></td>
                <td></td>
                <td>bexpr -> bterm bexpr'</td>
                <td>bexpr -> bterm bexpr'</td>
                <td></td>
                <td>bexpr -> bterm bexpr'</td>
                <td>bexpr -> bterm bexpr'</td>
                <td></td>
            </tr>
            <tr>
                <th>bexpr'</th>
                <td></td>
                <td>bexpr' -> or bterm bexpr'</td>
                <td></td>
                <td></td>
                <td>bexpr' -> ε</td>
                <td></td>
                <td></td>
                <
